examples/induction_test.v
@@ -1,0 +1,296 @@
+(* Add LoadPath "C:\Users\Ziga\Documents\Ziga_podatki\repositories\eeff-formalization\syntax". *)
+(* Add LoadPath "C:\Users\Ziga\Documents\Ziga_podatki\repositories\eeff-formalization\type_system". *)
+(* Add LoadPath "C:\Users\Ziga\Documents\Ziga_podatki\repositories\eeff-formalization\substitution". *)
+(* Add LoadPath "C:\Users\Ziga\Documents\Ziga_podatki\repositories\eeff-formalization\operational_semantics". *)
+(* Add LoadPath "C:\Users\Ziga\Documents\Ziga_podatki\repositories\eeff-formalization\logic". *)
+(* Add LoadPath "C:\Users\Ziga\Documents\Ziga_podatki\repositories\eeff-formalization\examples". *)
+Add LoadPath "E:\Ziga_Podatki\faks\eeff-formalization\syntax".
+Add LoadPath "E:\Ziga_Podatki\faks\eeff-formalization\type_system".
+Add LoadPath "E:\Ziga_Podatki\faks\eeff-formalization\substitution".
+Add LoadPath "E:\Ziga_Podatki\faks\eeff-formalization\operational_semantics".
+Add LoadPath "E:\Ziga_Podatki\faks\eeff-formalization\logic".
+Add LoadPath "E:\Ziga_Podatki\faks\eeff-formalization\examples".
+
+Require Export type_lemmas logic_lemmas logic_tactics.
+Open Scope string_scope.
+
+
+Lemma letbind_ctype A c1 c2 Γ D:
+  has_ctype Γ c1 (CTy A SigØ EqsØ) -> has_ctype (CtxU Γ A) c2 D ->
+  has_ctype Γ (DoBind c1 c2) D.
+Proof.
+intros tys1 tys2.
+apply TypeC. inv tys1. auto. inv tys2. auto.
+destruct D as [B Σ E]. eapply TypeDoBind; eauto.
+apply TypeC. inv tys1. auto.
++ apply WfCTy. inv tys1. inv H0. auto.
+  all: inv tys2; inv H0; auto.
++ eapply TypeCSubtype; eauto. apply SubtypeCTy.
+  apply vsubtype_refl. inv tys1. inv H0. auto.
+  apply SubtypeSigØ. apply SubtypeEqsØ.
+Qed.
+
+Lemma unpure_ret Γ A Σ E v:
+  wf_sig Σ -> wf_eqs E Σ -> has_vtype Γ v A ->
+  has_ctype Γ (Ret v) (CTy A Σ E).
+Proof.
+intros wfs wfe vty. apply TypeC. inv vty. auto. obvious. inv vty. auto.
+eapply TypeCSubtype. instantiate (1:= (CTy A SigØ EqsØ)).
+obvious_ctype. all: inv vty; auto. apply SubtypeCTy.
+apply vsubtype_refl. auto. apply SubtypeSigØ. apply SubtypeEqsØ.
+Qed.
+
+(* ========================================================================== *)
+
+
+Example etabind_with_induction Γ Ψ C c:
+  wf_ctype C -> wf_ctx Γ -> wf_hyp Γ Ψ -> has_ctype Γ c C ->
+  judg Γ Ψ (Ceq C (DoBind c (Ret (Var 0))) c).
+Proof.
+intros wfc wfg wfh ctys. destruct C as [A Σ E]. inv wfc.
+(* Translate arbitrary computation to arbitrary functions. *)
+assert (
+  judg Γ Ψ (Forall (TyFun TyUnit (CTy A Σ E))
+    (Ceq (CTy A Σ E) 
+      (DoBind (App (Var 0) Unit) (Ret (Var 0))) (App (Var 0) Unit)
+  ))).
+{ (* The showcase of induction. *)
+apply WfJudg; auto.
+{ apply WfForall; obvious. apply WfCeq.
+  + ctype_step. instantiate (1:=A). obvious_ctype.
+    apply unpure_ret; obvious_vtype.
+  + obvious_ctype. }
+apply CompInduction.
++ apply WfCeq. ctype_step. instantiate (1:=A). obvious_ctype.
+  apply unpure_ret; obvious_vtype. obvious_ctype.
++ (* Base Case *)
+  simpl. simpl_c_subs.
+  assert (wf_hyp (CtxU Γ A) (hyp_shift Ψ 1 0)) as wfhyp.
+  { apply wf_hyp_shift_typesafe; auto. }
+  
+  eapply ceq_trans. apply WfJudg; obvious. 2: eapply CeqDoBind.
+  3: apply ceq_refl. 2: apply WfJudg. 4: eapply βApp. all: auto.
+  apply WfCeq. 3: apply WfCeq.
+
+  { ctype_step. instantiate (1:=A). ctype_step. 2: obvious_vtype.
+    vtype_step. apply unpure_ret; obvious_vtype.
+    apply unpure_ret; obvious_vtype. }
+  { simpl_c_subs. ctype_step. instantiate (1:=A).
+    apply unpure_ret; obvious_vtype. apply unpure_ret; obvious_vtype. }
+  { instantiate (1:=A). ctype_step. 2:obvious_vtype.
+    vtype_step. apply unpure_ret; obvious_vtype. }
+  { simpl_c_subs. apply unpure_ret; obvious_vtype. }
+  { apply unpure_ret; obvious_vtype. }
+  { apply wf_hyp_shift_typesafe; auto. }
+
+  simpl_c_subs. eapply ceq_trans. apply WfJudg; auto. 2:eapply βDoBind_Ret.
+  all: simpl_c_subs. apply WfCeq.
+
+  { ctype_step. instantiate (1:=A). all: apply unpure_ret; obvious_vtype. }
+  { apply unpure_ret; obvious_vtype. }
+
+  eapply ceq_sym. eapply ceq_trans. apply WfJudg; auto. 2:eapply βApp.
+  all: simpl_c_subs. apply WfCeq.
+
+  { ctype_step. vtype_step. apply unpure_ret; obvious_vtype. obvious_vtype. }
+  { apply unpure_ret; obvious_vtype. }
+
+  eapply ceq_refl. apply unpure_ret; obvious_vtype. auto.
+
++ (* Step Case *)
+  intros op Aop Bop gets.
+  apply get_op_type_wf in gets as getss. destruct getss. 2: auto.
+  simpl. simpl_c_subs.
+
+  assert (
+    wf_hyp (CtxU (CtxU Γ Aop) (TyFun Bop (CTy A Σ E)))
+    (HypU (hyp_shift Ψ 2 0)
+     (Forall Bop (Ceq (CTy A Σ E)
+      (DoBind (App (Fun (App (Var 2) (Var 1))) Unit) (Ret (Var 0)))
+      (App (Fun (App (Var 2) (Var 1))) Unit)))) ) as wfhyp.
+  { apply WfHypU.
+    + rewrite <-(hyp_shift_shift 1). apply wf_hyp_shift_typesafe.
+      apply wf_hyp_shift_typesafe. all: obvious.
+    + apply WfForall. obvious. apply WfCeq.
+      - ctype_step. instantiate (1:=A). ctype_step. 2: obvious_vtype.
+        vtype_step. ctype_step. instantiate (1:=Bop). all: obvious_vtype.
+        apply unpure_ret; obvious_vtype.
+      - ctype_step. 2: obvious_vtype. vtype_step. ctype_step.
+        instantiate (1:=Bop). all:obvious_vtype. }
+  
+  eapply ceq_trans. apply WfJudg; obvious. 2: eapply CeqDoBind.
+  3: apply ceq_refl. 2: apply WfJudg. 4: eapply βApp. all: auto.
+  apply WfCeq. 3: apply WfCeq. all: simpl_c_subs.
+
+  { ctype_step. instantiate (1:=A). 2: apply unpure_ret; obvious_vtype.
+    ctype_step. 2: obvious_vtype. vtype_step. ctype_step.
+    eapply TypeOp; eauto. obvious_vtype. ctype_step.
+    instantiate (1:=Bop). all: obvious_vtype. }
+  { ctype_step. instantiate (1:=A). 2: apply unpure_ret; obvious_vtype.
+    ctype_step. eapply TypeOp; eauto. obvious_vtype. ctype_step.
+    instantiate (1:=Bop). all: obvious_vtype. }
+  { instantiate (1:=A). ctype_step. 2: obvious_vtype. vtype_step.
+    ctype_step. eapply TypeOp; eauto. obvious_vtype. ctype_step.
+    instantiate (1:=Bop). all: obvious_vtype. }
+  { ctype_step. eapply TypeOp; eauto. obvious_vtype. ctype_step.
+    instantiate (1:=Bop). all: obvious_vtype. }
+  { apply unpure_ret; obvious_vtype. }
+  { eapply wf_hyp_shift_typesafe in wfhyp. simpl in wfhyp. eauto. auto. }
+
+  eapply ceq_trans. apply WfJudg; obvious. 2: eapply βDoBind_Op.
+  all: simpl. apply WfCeq.
+
+  { ctype_step. instantiate (1:=A). ctype_step. eapply TypeOp; eauto.
+    obvious_vtype. ctype_step. instantiate (1:=Bop). all: obvious_vtype.
+    apply unpure_ret; obvious_vtype. }
+  { ctype_step. eapply TypeOp; eauto. obvious_vtype. ctype_step.
+    instantiate (1:=A). ctype_step. instantiate (1:=Bop). all: obvious_vtype.
+    apply unpure_ret; obvious_vtype. }
+
+  apply ceq_sym. eapply ceq_trans. apply WfJudg; obvious. 2: eapply βApp.
+  all: simpl_c_subs. apply WfCeq.
+
+  { ctype_step. 2: obvious_vtype. vtype_step. ctype_step. eapply TypeOp; eauto.
+    obvious_vtype. ctype_step. instantiate (1:=Bop). all: obvious_vtype. }
+  { ctype_step. eapply TypeOp; eauto.
+    obvious_vtype. ctype_step. instantiate (1:=Bop). all: obvious_vtype. }
+
+  apply ceq_sym. apply WfJudg; obvious. 2: eapply CeqOp; eauto.
+  2: apply veq_refl. apply WfCeq. 4: auto.
+
+  { ctype_step. eapply TypeOp; eauto. obvious_vtype.
+    ctype_step. instantiate (1:=A). ctype_step. instantiate (1:=Bop).
+    all: obvious_vtype. apply unpure_ret; obvious_vtype. }
+  { ctype_step. eapply TypeOp; eauto.
+    obvious_vtype. ctype_step. instantiate (1:=Bop). all: obvious_vtype. }
+  { obvious_vtype. }
+
+  assert (
+    judg (CtxU (CtxU Γ Aop) (TyFun Bop (CTy A Σ E)))
+      (HypU (hyp_shift Ψ 2 0)
+        (Forall Bop
+          (Ceq (CTy A Σ E)
+            (DoBind (App (Fun (App (Var 2) (Var 1))) Unit)
+             (Ret (Var 0))) (App (Fun (App (Var 2) (Var 1))) Unit))))
+      (Forall Bop
+        (Ceq (CTy A Σ E)
+            (DoBind (App (Fun (App (Var 2) (Var 1))) Unit)
+              (Ret (Var 0))) (App (Fun (App (Var 2) (Var 1))) Unit)))) as IH.
+  { apply WfJudg; auto.
+    apply WfForall; obvious. apply WfCeq. ctype_step. instantiate (1:=A).
+    ctype_step. 2:obvious_vtype. vtype_step. ctype_step. instantiate (1:=Bop).
+    all: obvious_vtype. apply unpure_ret; obvious_vtype.
+    ctype_step. vtype_step. ctype_step. instantiate (1:=Bop).
+    all: obvious_vtype.
+    apply IsHyp. simpl. left. auto. }
+  
+  eapply judg_shift_typesafe in IH. 2: exact H0. eapply ForallEl in IH.
+  2: instantiate (1:=(Var 0)); obvious_vtype. simpl in IH.
+  unfold c_subs in IH. simpl in IH. simpl.
+
+  assert (forall Ψ', 
+    wf_hyp (CtxU (CtxU (CtxU Γ Aop) (TyFun Bop (CTy A Σ E))) Bop) Ψ' ->
+    judg (CtxU (CtxU (CtxU Γ Aop) (TyFun Bop (CTy A Σ E))) Bop) Ψ'
+       (Ceq (CTy A Σ E)
+          (DoBind (App (Fun (App (Var 2) (Var 1))) Unit) (Ret (Var 0)))
+          (DoBind (App (Var 1) (Var 0)) (Ret (Var 0))))) as IH1.
+  { clear wfhyp IH. intros Ψ' wfh'.
+    apply WfJudg; auto. apply WfCeq.
+    3: eapply CeqDoBind. 3: instantiate (1:=A). 4: apply ceq_refl.
+    3: eapply ceq_trans. 3: eapply WfJudg; auto. 4: apply βApp.
+    + ctype_step. instantiate (1:=A). ctype_step. 2: obvious_vtype.
+      vtype_step. ctype_step. instantiate (1:=Bop). all: obvious_vtype.
+      apply unpure_ret; obvious_vtype.
+    + ctype_step. instantiate (1:=A). ctype_step. instantiate (1:=Bop).
+      all: obvious_vtype. apply unpure_ret; obvious_vtype.
+    + simpl_c_subs. apply WfCeq. ctype_step. 2:obvious_vtype.
+      vtype_step. ctype_step. instantiate (1:=Bop). all: obvious_vtype.
+      ctype_step. instantiate (1:=Bop). all: obvious_vtype.
+    + simpl_c_subs. apply ceq_refl; auto. ctype_step.
+      instantiate (1:=Bop). all: obvious_vtype.
+    + apply unpure_ret; obvious_vtype.
+    + eapply wf_hyp_shift_typesafe in wfh'; eauto. }
+
+  eapply ceq_sym in IH1. 
+  2: eapply wf_hyp_shift_typesafe in wfhyp; eauto.
+  eapply ceq_trans. eauto. clear IH1.
+  
+  assert (forall Ψ', 
+    wf_hyp (CtxU (CtxU (CtxU Γ Aop) (TyFun Bop (CTy A Σ E))) Bop) Ψ' ->
+    judg (CtxU (CtxU (CtxU Γ Aop) (TyFun Bop (CTy A Σ E))) Bop) Ψ'
+       (Ceq (CTy A Σ E)
+          (App (Fun (App (Var 2) (Var 1))) Unit)
+          (App (Var 1) (Var 0)))) as IH1.
+  { clear wfhyp IH. intros Ψ' wfh'. eapply ceq_trans. apply WfJudg; auto.
+    2: apply βApp. all: simpl_c_subs. apply WfCeq.
+    3: apply ceq_refl; auto.
+    + ctype_step. 2: obvious_vtype. vtype_step. ctype_step.
+      instantiate (1:=Bop). all: obvious_vtype.
+    + ctype_step. instantiate (1:=Bop). all: obvious_vtype.
+    + ctype_step. instantiate (1:=Bop). all: obvious_vtype. }
+  
+  eapply ceq_sym. eapply ceq_sym in IH1.
+  2: eapply wf_hyp_shift_typesafe in wfhyp; eauto.
+  eapply ceq_trans. eauto. clear IH1. apply ceq_sym.
+  eapply WfJudg; auto. eapply WfCeq.
+
+  { ctype_step. instantiate (1:=A). ctype_step. 2: obvious_vtype.
+    vtype_step. ctype_step. instantiate (1:=Bop). 2: obvious_vtype.
+    all: obvious_vtype. apply unpure_ret; obvious_vtype. }
+  { ctype_step. 2: obvious_vtype. vtype_step. ctype_step.
+    instantiate (1:=Bop). all: obvious_vtype. }
+  { eapply wf_hyp_shift_typesafe in wfhyp; eauto. }
+}{
+(* Now lets put induction to good use *)
+eapply ForallEl in H.
+Focus 2.
+  instantiate (1:= (Fun (c_shift c 1 0))).
+  vtype_step. apply c_shift_typesafe; obvious.
+simpl in H. unfold c_subs in H. simpl in H. 
+rewrite c_negshift_shift, c_shift_0 in H. 2: omega.
+
+assert (
+  judg Γ Ψ
+      (Ceq (CTy A Σ E)
+         (DoBind (App (Fun (c_shift c 1 0)) Unit) (Ret (Var 0)))
+         (App (Fun (c_shift c 1 0)) Unit)) ) as IH.
+{ apply WfJudg; auto. apply WfCeq. ctype_step. instantiate (1:=A).
+  obvious_ctype. apply TypeFun. apply c_shift_typesafe; obvious.
+  apply unpure_ret; obvious_vtype. obvious_ctype. apply TypeFun.
+  apply c_shift_typesafe; obvious. }
+
+assert (
+  judg Γ Ψ
+    (Ceq (CTy A Σ E)
+      (DoBind (App (Fun (c_shift c 1 0)) Unit) (Ret (Var 0)))
+      (DoBind c (Ret (Var 0))) )) as IH1.
+{ eapply ceq_trans. apply WfJudg; auto. 2: eapply CeqDoBind.
+  3: apply ceq_refl. 2: instantiate (2:=A). 2: apply WfJudg; auto.
+  3: apply βApp. apply WfCeq. 3: apply WfCeq. 
+  + ctype_step. instantiate (1:=A). obvious_ctype. apply TypeFun.
+    apply c_shift_typesafe; obvious. apply unpure_ret; obvious_vtype.
+  + ctype_step. eapply c_subs_typesafe. apply c_shift_typesafe. eauto.
+    2: obvious_vtype. 3: omega. obvious. destruct Γ; simpl; auto.
+    apply unpure_ret; obvious_vtype.
+  + ctype_step. vtype_step. apply c_shift_typesafe. all: obvious_vtype.
+  + eapply c_subs_typesafe. apply c_shift_typesafe. eauto.
+    2: obvious_vtype. 3: omega. obvious. destruct Γ; simpl; auto.
+  + apply unpure_ret; obvious_vtype.
+  + apply wf_hyp_shift_typesafe; auto.
+  + simpl_c_subs. rewrite c_sub_no_var_same, c_negshift_shift, c_shift_0.
+    apply ceq_refl. ctype_step. eauto. apply unpure_ret; obvious_vtype.
+    all: aomega. apply c_shift_makes_no_var. }
+
+assert (
+  judg Γ Ψ (Ceq (CTy A Σ E) (App (Fun (c_shift c 1 0)) Unit) c) ) as IH2.
+{ eapply ceq_trans. apply WfJudg; auto. 2: eapply βApp.
+  all: simpl_c_subs; rewrite c_sub_no_var_same, c_negshift_shift, c_shift_0.
+  2: omega. 4:omega. all: try apply c_shift_makes_no_var.
+  apply WfCeq. 3: apply ceq_refl. all: auto.
+  obvious_ctype. apply TypeFun. apply c_shift_typesafe; obvious. }
+
+eapply ceq_trans. apply ceq_sym. eauto.
+apply ceq_sym. eapply ceq_trans. apply ceq_sym. eauto.
+apply ceq_sym. auto.
+}
+Qed.
